cube

code/ecdsap256sha2/Hacl.Impl.P256.Arithmetics.fst
@@ -24,6 +24,32 @@ open FStar.Mul
 
 #reset-options "--z3rlimit 100" 
 
+val cube: a: felem -> result: felem -> Stack unit
+  (requires fun h -> live h a /\ live h result /\ disjoint a result /\ as_nat h a < prime)
+  (ensures fun h0 _ h1 -> modifies (loc result) h0 h1 /\ 
+    as_nat h1 result = toDomain_ (fromDomain_ (as_nat h0 a) * fromDomain_ (as_nat h0 a) * fromDomain_ (as_nat h0 a) % prime256) /\ 
+    as_nat h1 result = toDomain_ (fromDomain_ (as_nat h0 a) * fromDomain_ (as_nat h0 a) * fromDomain_ (as_nat h0 a)))
+
+
+let cube a result = 
+  let h0 = ST.get() in 
+    montgomery_multiplication_buffer a a result;
+    montgomery_multiplication_buffer result a result;
+ let h1 = ST.get() in 
+
+   calc (==) {
+     as_nat h1 result;
+     (==) {}
+     toDomain_ ((fromDomain_ (as_nat h0 a)  * fromDomain_ (as_nat h0 a) % prime256) * fromDomain_ (as_nat h0 a) % prime256);
+     (==) 
+       {
+	 lemma_mod_mul_distr_l (fromDomain_ (as_nat h0 a) * fromDomain_ (as_nat h0 a)) (fromDomain_ (as_nat h0 a)) prime256}
+     toDomain_ (fromDomain_ (as_nat h0 a) * fromDomain_ (as_nat h0 a) * fromDomain_ (as_nat h0 a) % prime256); };
+
+     inDomain_mod_is_not_mod (fromDomain_ (as_nat h0 a) * fromDomain_ (as_nat h0 a) * fromDomain_ (as_nat h0 a))
+
+
+
 let quatre a result = 
     let h0 = ST.get() in 
   montgomery_multiplication_buffer a a result;
